src/HOL/Wfrec.thy
@@ -7,20 +7,20 @@
 section \<open>Well-Founded Recursion Combinator\<close>
 
 theory Wfrec
-imports Wellfounded
+  imports Wellfounded
 begin
 
-inductive wfrec_rel :: "('a \<times> 'a) set \<Rightarrow> (('a \<Rightarrow> 'b) \<Rightarrow> ('a \<Rightarrow> 'b)) \<Rightarrow> 'a \<Rightarrow> 'b \<Rightarrow> bool" for R F where
-  wfrecI: "(\<And>z. (z, x) \<in> R \<Longrightarrow> wfrec_rel R F z (g z)) \<Longrightarrow> wfrec_rel R F x (F g x)"
+inductive wfrec_rel :: "('a \<times> 'a) set \<Rightarrow> (('a \<Rightarrow> 'b) \<Rightarrow> ('a \<Rightarrow> 'b)) \<Rightarrow> 'a \<Rightarrow> 'b \<Rightarrow> bool" for R F
+  where wfrecI: "(\<And>z. (z, x) \<in> R \<Longrightarrow> wfrec_rel R F z (g z)) \<Longrightarrow> wfrec_rel R F x (F g x)"
 
-definition cut :: "('a \<Rightarrow> 'b) \<Rightarrow> ('a \<times> 'a) set \<Rightarrow> 'a \<Rightarrow> 'a \<Rightarrow> 'b" where
-  "cut f R x = (\<lambda>y. if (y, x) \<in> R then f y else undefined)"
+definition cut :: "('a \<Rightarrow> 'b) \<Rightarrow> ('a \<times> 'a) set \<Rightarrow> 'a \<Rightarrow> 'a \<Rightarrow> 'b"
+  where "cut f R x = (\<lambda>y. if (y, x) \<in> R then f y else undefined)"
 
-definition adm_wf :: "('a \<times> 'a) set \<Rightarrow> (('a \<Rightarrow> 'b) \<Rightarrow> ('a \<Rightarrow> 'b)) \<Rightarrow> bool" where
-  "adm_wf R F \<longleftrightarrow> (\<forall>f g x. (\<forall>z. (z, x) \<in> R \<longrightarrow> f z = g z) \<longrightarrow> F f x = F g x)"
+definition adm_wf :: "('a \<times> 'a) set \<Rightarrow> (('a \<Rightarrow> 'b) \<Rightarrow> ('a \<Rightarrow> 'b)) \<Rightarrow> bool"
+  where "adm_wf R F \<longleftrightarrow> (\<forall>f g x. (\<forall>z. (z, x) \<in> R \<longrightarrow> f z = g z) \<longrightarrow> F f x = F g x)"
 
-definition wfrec :: "('a \<times> 'a) set \<Rightarrow> (('a \<Rightarrow> 'b) \<Rightarrow> ('a \<Rightarrow> 'b)) \<Rightarrow> ('a \<Rightarrow> 'b)" where
-  "wfrec R F = (\<lambda>x. THE y. wfrec_rel R (\<lambda>f x. F (cut f R x) x) x y)"
+definition wfrec :: "('a \<times> 'a) set \<Rightarrow> (('a \<Rightarrow> 'b) \<Rightarrow> ('a \<Rightarrow> 'b)) \<Rightarrow> ('a \<Rightarrow> 'b)"
+  where "wfrec R F = (\<lambda>x. THE y. wfrec_rel R (\<lambda>f x. F (cut f R x) x) x y)"
 
 lemma cuts_eq: "(cut f R x = cut g R x) \<longleftrightarrow> (\<forall>y. (y, x) \<in> R \<longrightarrow> f y = g y)"
   by (simp add: fun_eq_iff cut_def)
@@ -28,13 +28,17 @@ lemma cuts_eq: "(cut f R x = cut g R x) \<longleftrightarrow> (\<forall>y. (y, x
 lemma cut_apply: "(x, a) \<in> R \<Longrightarrow> cut f R a x = f x"
   by (simp add: cut_def)
 
-text\<open>Inductive characterization of wfrec combinator; for details see:
-John Harrison, "Inductive definitions: automation and application"\<close>
+text \<open>
+  Inductive characterization of \<open>wfrec\<close> combinator; for details see:
+  John Harrison, "Inductive definitions: automation and application".
+\<close>
 
 lemma theI_unique: "\<exists>!x. P x \<Longrightarrow> P x \<longleftrightarrow> x = The P"
   by (auto intro: the_equality[symmetric] theI)
 
-lemma wfrec_unique: assumes "adm_wf R F" "wf R" shows "\<exists>!y. wfrec_rel R F x y"
+lemma wfrec_unique:
+  assumes "adm_wf R F" "wf R"
+  shows "\<exists>!y. wfrec_rel R F x y"
   using \<open>wf R\<close>
 proof induct
   define f where "f y = (THE z. wfrec_rel R F y z)" for y
@@ -46,44 +50,46 @@ proof induct
 qed
 
 lemma adm_lemma: "adm_wf R (\<lambda>f x. F (cut f R x) x)"
-  by (auto simp add: adm_wf_def
-           intro!: arg_cong[where f="\<lambda>x. F x y" for y] cuts_eq[THEN iffD2])
+  by (auto simp: adm_wf_def intro!: arg_cong[where f="\<lambda>x. F x y" for y] cuts_eq[THEN iffD2])
 
 lemma wfrec: "wf R \<Longrightarrow> wfrec R F a = F (cut (wfrec R F) R a) a"
-apply (simp add: wfrec_def)
-apply (rule adm_lemma [THEN wfrec_unique, THEN the1_equality], assumption)
-apply (rule wfrec_rel.wfrecI)
-apply (erule adm_lemma [THEN wfrec_unique, THEN theI'])
-done
+  apply (simp add: wfrec_def)
+  apply (rule adm_lemma [THEN wfrec_unique, THEN the1_equality])
+   apply assumption
+  apply (rule wfrec_rel.wfrecI)
+  apply (erule adm_lemma [THEN wfrec_unique, THEN theI'])
+  done
 
 
-text\<open>* This form avoids giant explosions in proofs.  NOTE USE OF ==\<close>
+text \<open>This form avoids giant explosions in proofs.  NOTE USE OF \<open>\<equiv>\<close>.\<close>
 lemma def_wfrec: "f \<equiv> wfrec R F \<Longrightarrow> wf R \<Longrightarrow> f a = F (cut f R a) a"
- by (auto intro: wfrec)
+  by (auto intro: wfrec)
 
 
 subsubsection \<open>Well-founded recursion via genuine fixpoints\<close>
 
 lemma wfrec_fixpoint:
-  assumes WF: "wf R" and ADM: "adm_wf R F"
+  assumes wf: "wf R"
+    and adm: "adm_wf R F"
   shows "wfrec R F = F (wfrec R F)"
 proof (rule ext)
   fix x
   have "wfrec R F x = F (cut (wfrec R F) R x) x"
-    using wfrec[of R F] WF by simp
+    using wfrec[of R F] wf by simp
   also
-  { have "\<And> y. (y,x) \<in> R \<Longrightarrow> (cut (wfrec R F) R x) y = (wfrec R F) y"
-      by (auto simp add: cut_apply)
-    hence "F (cut (wfrec R F) R x) x = F (wfrec R F) x"
-      using ADM adm_wf_def[of R F] by auto }
+  have "\<And>y. (y, x) \<in> R \<Longrightarrow> cut (wfrec R F) R x y = wfrec R F y"
+    by (auto simp add: cut_apply)
+  then have "F (cut (wfrec R F) R x) x = F (wfrec R F) x"
+    using adm adm_wf_def[of R F] by auto
   finally show "wfrec R F x = F (wfrec R F) x" .
 qed
 
+
 subsection \<open>Wellfoundedness of \<open>same_fst\<close>\<close>
 
-definition same_fst :: "('a \<Rightarrow> bool) \<Rightarrow> ('a \<Rightarrow> ('b \<times> 'b) set) \<Rightarrow> (('a \<times> 'b) \<times> ('a \<times> 'b)) set" where
-  "same_fst P R = {((x', y'), (x, y)) . x' = x \<and> P x \<and> (y',y) \<in> R x}"
-   \<comment>\<open>For @{const wfrec} declarations where the first n parameters
+definition same_fst :: "('a \<Rightarrow> bool) \<Rightarrow> ('a \<Rightarrow> ('b \<times> 'b) set) \<Rightarrow> (('a \<times> 'b) \<times> ('a \<times> 'b)) set"
+  where "same_fst P R = {((x', y'), (x, y)) . x' = x \<and> P x \<and> (y',y) \<in> R x}"
+   \<comment> \<open>For @{const wfrec} declarations where the first n parameters
        stay unchanged in the recursive call.\<close>
 
 lemma same_fstI [intro!]: "P x \<Longrightarrow> (y', y) \<in> R x \<Longrightarrow> ((x, y'), (x, y)) \<in> same_fst P R"
@@ -92,12 +98,13 @@ lemma same_fstI [intro!]: "P x \<Longrightarrow> (y', y) \<in> R x \<Longrightar
 lemma wf_same_fst:
   assumes prem: "\<And>x. P x \<Longrightarrow> wf (R x)"
   shows "wf (same_fst P R)"
-apply (simp cong del: imp_cong add: wf_def same_fst_def)
-apply (intro strip)
-apply (rename_tac a b)
-apply (case_tac "wf (R a)")
- apply (erule_tac a = b in wf_induct, blast)
-apply (blast intro: prem)
-done
+  apply (simp cong del: imp_cong add: wf_def same_fst_def)
+  apply (intro strip)
+  apply (rename_tac a b)
+  apply (case_tac "wf (R a)")
+   apply (erule_tac a = b in wf_induct)
+   apply blast
+  apply (blast intro: prem)
+  done
 
 end
