src/HOL/Order_Relation.thy
@@ -9,7 +9,7 @@ theory Order_Relation
 imports Wfrec
 begin
 
-subsection\<open>Orders on a set\<close>
+subsection \<open>Orders on a set\<close>
 
 definition "preorder_on A r \<equiv> refl_on A r \<and> trans r"
 
@@ -27,51 +27,48 @@ lemmas order_on_defs =
 
 
 lemma preorder_on_empty[simp]: "preorder_on {} {}"
-by(simp add:preorder_on_def trans_def)
+  by (simp add: preorder_on_def trans_def)
 
 lemma partial_order_on_empty[simp]: "partial_order_on {} {}"
-by(simp add:partial_order_on_def)
+  by (simp add: partial_order_on_def)
 
 lemma lnear_order_on_empty[simp]: "linear_order_on {} {}"
-by(simp add:linear_order_on_def)
+  by (simp add: linear_order_on_def)
 
 lemma well_order_on_empty[simp]: "well_order_on {} {}"
-by(simp add:well_order_on_def)
+  by (simp add: well_order_on_def)
 
 
-lemma preorder_on_converse[simp]: "preorder_on A (r^-1) = preorder_on A r"
-by (simp add:preorder_on_def)
+lemma preorder_on_converse[simp]: "preorder_on A (r\<inverse>) = preorder_on A r"
+  by (simp add: preorder_on_def)
 
-lemma partial_order_on_converse[simp]:
-  "partial_order_on A (r^-1) = partial_order_on A r"
-by (simp add: partial_order_on_def)
+lemma partial_order_on_converse[simp]: "partial_order_on A (r\<inverse>) = partial_order_on A r"
+  by (simp add: partial_order_on_def)
 
-lemma linear_order_on_converse[simp]:
-  "linear_order_on A (r^-1) = linear_order_on A r"
-by (simp add: linear_order_on_def)
+lemma linear_order_on_converse[simp]: "linear_order_on A (r\<inverse>) = linear_order_on A r"
+  by (simp add: linear_order_on_def)
 
 
-lemma strict_linear_order_on_diff_Id:
-  "linear_order_on A r \<Longrightarrow> strict_linear_order_on A (r-Id)"
-by(simp add: order_on_defs trans_diff_Id)
+lemma strict_linear_order_on_diff_Id: "linear_order_on A r \<Longrightarrow> strict_linear_order_on A (r - Id)"
+  by (simp add: order_on_defs trans_diff_Id)
 
 lemma linear_order_on_singleton [simp]: "linear_order_on {x} {(x, x)}"
-unfolding order_on_defs by simp
+  by (simp add: order_on_defs)
 
 lemma linear_order_on_acyclic:
   assumes "linear_order_on A r"
   shows "acyclic (r - Id)"
-using strict_linear_order_on_diff_Id[OF assms] 
-by(auto simp add: acyclic_irrefl strict_linear_order_on_def)
+  using strict_linear_order_on_diff_Id[OF assms]
+  by (auto simp add: acyclic_irrefl strict_linear_order_on_def)
 
 lemma linear_order_on_well_order_on:
   assumes "finite r"
   shows "linear_order_on A r \<longleftrightarrow> well_order_on A r"
-unfolding well_order_on_def
-using assms finite_acyclic_wf[OF _ linear_order_on_acyclic, of r] by blast
+  unfolding well_order_on_def
+  using assms finite_acyclic_wf[OF _ linear_order_on_acyclic, of r] by blast
 
 
-subsection\<open>Orders on the field\<close>
+subsection \<open>Orders on the field\<close>
 
 abbreviation "Refl r \<equiv> refl_on (Field r) r"
 
@@ -87,50 +84,57 @@ abbreviation "Well_order r \<equiv> well_order_on (Field r) r"
 
 
 lemma subset_Image_Image_iff:
-  "\<lbrakk> Preorder r; A \<subseteq> Field r; B \<subseteq> Field r\<rbrakk> \<Longrightarrow>
-   r `` A \<subseteq> r `` B \<longleftrightarrow> (\<forall>a\<in>A.\<exists>b\<in>B. (b,a):r)"
-unfolding preorder_on_def refl_on_def Image_def
-apply (simp add: subset_eq)
-unfolding trans_def by fast
+  "Preorder r \<Longrightarrow> A \<subseteq> Field r \<Longrightarrow> B \<subseteq> Field r \<Longrightarrow>
+    r `` A \<subseteq> r `` B \<longleftrightarrow> (\<forall>a\<in>A.\<exists>b\<in>B. (b, a) \<in> r)"
+  apply (simp add: preorder_on_def refl_on_def Image_def subset_eq)
+  apply (simp only: trans_def)
+  apply fast
+  done
 
 lemma subset_Image1_Image1_iff:
-  "\<lbrakk> Preorder r; a : Field r; b : Field r\<rbrakk> \<Longrightarrow> r `` {a} \<subseteq> r `` {b} \<longleftrightarrow> (b,a):r"
-by(simp add:subset_Image_Image_iff)
+  "Preorder r \<Longrightarrow> a \<in> Field r \<Longrightarrow> b \<in> Field r \<Longrightarrow> r `` {a} \<subseteq> r `` {b} \<longleftrightarrow> (b, a) \<in> r"
+  by (simp add: subset_Image_Image_iff)
 
 lemma Refl_antisym_eq_Image1_Image1_iff:
-  assumes r: "Refl r" and as: "antisym r" and abf: "a \<in> Field r" "b \<in> Field r"
+  assumes "Refl r"
+    and as: "antisym r"
+    and abf: "a \<in> Field r" "b \<in> Field r"
   shows "r `` {a} = r `` {b} \<longleftrightarrow> a = b"
+    (is "?lhs \<longleftrightarrow> ?rhs")
 proof
-  assume "r `` {a} = r `` {b}"
-  hence e: "\<And>x. (a, x) \<in> r \<longleftrightarrow> (b, x) \<in> r" by (simp add: set_eq_iff)
-  have "(a, a) \<in> r" "(b, b) \<in> r" using r abf by (simp_all add: refl_on_def)
-  hence "(a, b) \<in> r" "(b, a) \<in> r" using e[of a] e[of b] by simp_all
-  thus "a = b" using as[unfolded antisym_def] by blast
-qed fast
+  assume ?lhs
+  then have *: "\<And>x. (a, x) \<in> r \<longleftrightarrow> (b, x) \<in> r"
+    by (simp add: set_eq_iff)
+  have "(a, a) \<in> r" "(b, b) \<in> r" using \<open>Refl r\<close> abf by (simp_all add: refl_on_def)
+  then have "(a, b) \<in> r" "(b, a) \<in> r" using *[of a] *[of b] by simp_all
+  then show ?rhs
+    using \<open>antisym r\<close>[unfolded antisym_def] by blast
+next
+  assume ?rhs
+  then show ?lhs by fast
+qed
 
 lemma Partial_order_eq_Image1_Image1_iff:
-  "\<lbrakk>Partial_order r; a:Field r; b:Field r\<rbrakk> \<Longrightarrow> r `` {a} = r `` {b} \<longleftrightarrow> a=b"
-by(auto simp:order_on_defs Refl_antisym_eq_Image1_Image1_iff)
+  "Partial_order r \<Longrightarrow> a \<in> Field r \<Longrightarrow> b \<in> Field r \<Longrightarrow> r `` {a} = r `` {b} \<longleftrightarrow> a = b"
+  by (auto simp: order_on_defs Refl_antisym_eq_Image1_Image1_iff)
 
 lemma Total_Id_Field:
-assumes TOT: "Total r" and NID: "\<not> (r <= Id)"
-shows "Field r = Field(r - Id)"
-using mono_Field[of "r - Id" r] Diff_subset[of r Id]
-proof(auto)
-  have "r \<noteq> {}" using NID by fast
-  then obtain b and c where "b \<noteq> c \<and> (b,c) \<in> r" using NID by auto
-  hence 1: "b \<noteq> c \<and> {b,c} \<le> Field r" by (auto simp: Field_def)
-
+  assumes "Total r"
+    and not_Id: "\<not> r \<subseteq> Id"
+  shows "Field r = Field (r - Id)"
+  using mono_Field[of "r - Id" r] Diff_subset[of r Id]
+proof auto
   fix a assume *: "a \<in> Field r"
-  obtain d where 2: "d \<in> Field r" and 3: "d \<noteq> a"
-  using * 1 by auto
-  hence "(a,d) \<in> r \<or> (d,a) \<in> r" using * TOT
-  by (simp add: total_on_def)
-  thus "a \<in> Field(r - Id)" using 3 unfolding Field_def by blast
+  from not_Id have "r \<noteq> {}" by fast
+  with not_Id obtain b and c where "b \<noteq> c \<and> (b,c) \<in> r" by auto
+  then have "b \<noteq> c \<and> {b, c} \<subseteq> Field r" by (auto simp: Field_def)
+  with * obtain d where "d \<in> Field r" "d \<noteq> a" by auto
+  with * \<open>Total r\<close> have "(a, d) \<in> r \<or> (d, a) \<in> r" by (simp add: total_on_def)
+  with \<open>d \<noteq> a\<close> show "a \<in> Field (r - Id)" unfolding Field_def by blast
 qed
 
 
-subsection\<open>Orders on a type\<close>
+subsection \<open>Orders on a type\<close>
 
 abbreviation "strict_linear_order \<equiv> strict_linear_order_on UNIV"
 
@@ -141,297 +145,303 @@ abbreviation "well_order \<equiv> well_order_on UNIV"
 
 subsection \<open>Order-like relations\<close>
 
-text\<open>In this subsection, we develop basic concepts and results pertaining
-to order-like relations, i.e., to reflexive and/or transitive and/or symmetric and/or
-total relations. We also further define upper and lower bounds operators.\<close>
+text \<open>
+  In this subsection, we develop basic concepts and results pertaining
+  to order-like relations, i.e., to reflexive and/or transitive and/or symmetric and/or
+  total relations. We also further define upper and lower bounds operators.
+\<close>
 
 
 subsubsection \<open>Auxiliaries\<close>
 
-lemma refl_on_domain:
-"\<lbrakk>refl_on A r; (a,b) : r\<rbrakk> \<Longrightarrow> a \<in> A \<and> b \<in> A"
-by(auto simp add: refl_on_def)
+lemma refl_on_domain: "refl_on A r \<Longrightarrow> (a, b) \<in> r \<Longrightarrow> a \<in> A \<and> b \<in> A"
+  by (auto simp add: refl_on_def)
 
-corollary well_order_on_domain:
-"\<lbrakk>well_order_on A r; (a,b) \<in> r\<rbrakk> \<Longrightarrow> a \<in> A \<and> b \<in> A"
-by (auto simp add: refl_on_domain order_on_defs)
+corollary well_order_on_domain: "well_order_on A r \<Longrightarrow> (a, b) \<in> r \<Longrightarrow> a \<in> A \<and> b \<in> A"
+  by (auto simp add: refl_on_domain order_on_defs)
 
-lemma well_order_on_Field:
-"well_order_on A r \<Longrightarrow> A = Field r"
-by(auto simp add: refl_on_def Field_def order_on_defs)
+lemma well_order_on_Field: "well_order_on A r \<Longrightarrow> A = Field r"
+  by (auto simp add: refl_on_def Field_def order_on_defs)
 
-lemma well_order_on_Well_order:
-"well_order_on A r \<Longrightarrow> A = Field r \<and> Well_order r"
-using well_order_on_Field by auto
+lemma well_order_on_Well_order: "well_order_on A r \<Longrightarrow> A = Field r \<and> Well_order r"
+  using well_order_on_Field [of A] by auto
 
 lemma Total_subset_Id:
-assumes TOT: "Total r" and SUB: "r \<le> Id"
-shows "r = {} \<or> (\<exists>a. r = {(a,a)})"
-proof-
-  {assume "r \<noteq> {}"
-   then obtain a b where 1: "(a,b) \<in> r" by fast
-   hence "a = b" using SUB by blast
-   hence 2: "(a,a) \<in> r" using 1 by simp
-   {fix c d assume "(c,d) \<in> r"
-    hence "{a,c,d} \<le> Field r" using 1 unfolding Field_def by blast
-    hence "((a,c) \<in> r \<or> (c,a) \<in> r \<or> a = c) \<and>
-           ((a,d) \<in> r \<or> (d,a) \<in> r \<or> a = d)"
-    using TOT unfolding total_on_def by blast
-    hence "a = c \<and> a = d" using SUB by blast
-   }
-   hence "r \<le> {(a,a)}" by auto
-   with 2 have "\<exists>a. r = {(a,a)}" by blast
-  }
-  thus ?thesis by blast
+  assumes "Total r"
+    and "r \<subseteq> Id"
+  shows "r = {} \<or> (\<exists>a. r = {(a, a)})"
+proof -
+  have "\<exists>a. r = {(a, a)}" if "r \<noteq> {}"
+  proof -
+    from that obtain a b where ab: "(a, b) \<in> r" by fast
+    with \<open>r \<subseteq> Id\<close> have "a = b" by blast
+    with ab have aa: "(a, a) \<in> r" by simp
+    have "a = c \<and> a = d" if "(c, d) \<in> r" for c d
+    proof -
+      from that have "{a, c, d} \<subseteq> Field r"
+        using ab unfolding Field_def by blast
+      then have "((a, c) \<in> r \<or> (c, a) \<in> r \<or> a = c) \<and> ((a, d) \<in> r \<or> (d, a) \<in> r \<or> a = d)"
+        using \<open>Total r\<close> unfolding total_on_def by blast
+      with \<open>r \<subseteq> Id\<close> show ?thesis by blast
+    qed
+    then have "r \<subseteq> {(a, a)}" by auto
+    with aa show ?thesis by blast
+  qed
+  then show ?thesis by blast
 qed
 
 lemma Linear_order_in_diff_Id:
-assumes LI: "Linear_order r" and
-        IN1: "a \<in> Field r" and IN2: "b \<in> Field r"
-shows "((a,b) \<in> r) = ((b,a) \<notin> r - Id)"
-using assms unfolding order_on_defs total_on_def antisym_def Id_def refl_on_def by force
+  assumes "Linear_order r"
+    and "a \<in> Field r"
+    and "b \<in> Field r"
+  shows "(a, b) \<in> r \<longleftrightarrow> (b, a) \<notin> r - Id"
+  using assms unfolding order_on_defs total_on_def antisym_def Id_def refl_on_def by force
 
 
 subsubsection \<open>The upper and lower bounds operators\<close>
 
-text\<open>Here we define upper (``above") and lower (``below") bounds operators.
-We think of \<open>r\<close> as a {\em non-strict} relation.  The suffix ``S"
-at the names of some operators indicates that the bounds are strict -- e.g.,
-\<open>underS a\<close> is the set of all strict lower bounds of \<open>a\<close> (w.r.t. \<open>r\<close>).
-Capitalization of the first letter in the name reminds that the operator acts on sets, rather
-than on individual elements.\<close>
+text \<open>
+  Here we define upper (``above") and lower (``below") bounds operators. We
+  think of \<open>r\<close> as a \<^emph>\<open>non-strict\<close> relation. The suffix \<open>S\<close> at the names of
+  some operators indicates that the bounds are strict -- e.g., \<open>underS a\<close> is
+  the set of all strict lower bounds of \<open>a\<close> (w.r.t. \<open>r\<close>). Capitalization of
+  the first letter in the name reminds that the operator acts on sets, rather
+  than on individual elements.
+\<close>
 
-definition under::"'a rel \<Rightarrow> 'a \<Rightarrow> 'a set"
-where "under r a \<equiv> {b. (b,a) \<in> r}"
+definition under :: "'a rel \<Rightarrow> 'a \<Rightarrow> 'a set"
+  where "under r a \<equiv> {b. (b, a) \<in> r}"
 
-definition underS::"'a rel \<Rightarrow> 'a \<Rightarrow> 'a set"
-where "underS r a \<equiv> {b. b \<noteq> a \<and> (b,a) \<in> r}"
+definition underS :: "'a rel \<Rightarrow> 'a \<Rightarrow> 'a set"
+  where "underS r a \<equiv> {b. b \<noteq> a \<and> (b, a) \<in> r}"
 
-definition Under::"'a rel \<Rightarrow> 'a set \<Rightarrow> 'a set"
-where "Under r A \<equiv> {b \<in> Field r. \<forall>a \<in> A. (b,a) \<in> r}"
+definition Under :: "'a rel \<Rightarrow> 'a set \<Rightarrow> 'a set"
+  where "Under r A \<equiv> {b \<in> Field r. \<forall>a \<in> A. (b, a) \<in> r}"
 
-definition UnderS::"'a rel \<Rightarrow> 'a set \<Rightarrow> 'a set"
-where "UnderS r A \<equiv> {b \<in> Field r. \<forall>a \<in> A. b \<noteq> a \<and> (b,a) \<in> r}"
+definition UnderS :: "'a rel \<Rightarrow> 'a set \<Rightarrow> 'a set"
+  where "UnderS r A \<equiv> {b \<in> Field r. \<forall>a \<in> A. b \<noteq> a \<and> (b, a) \<in> r}"
 
-definition above::"'a rel \<Rightarrow> 'a \<Rightarrow> 'a set"
-where "above r a \<equiv> {b. (a,b) \<in> r}"
+definition above :: "'a rel \<Rightarrow> 'a \<Rightarrow> 'a set"
+  where "above r a \<equiv> {b. (a, b) \<in> r}"
 
-definition aboveS::"'a rel \<Rightarrow> 'a \<Rightarrow> 'a set"
-where "aboveS r a \<equiv> {b. b \<noteq> a \<and> (a,b) \<in> r}"
+definition aboveS :: "'a rel \<Rightarrow> 'a \<Rightarrow> 'a set"
+  where "aboveS r a \<equiv> {b. b \<noteq> a \<and> (a, b) \<in> r}"
 
-definition Above::"'a rel \<Rightarrow> 'a set \<Rightarrow> 'a set"
-where "Above r A \<equiv> {b \<in> Field r. \<forall>a \<in> A. (a,b) \<in> r}"
+definition Above :: "'a rel \<Rightarrow> 'a set \<Rightarrow> 'a set"
+  where "Above r A \<equiv> {b \<in> Field r. \<forall>a \<in> A. (a, b) \<in> r}"
 
-definition AboveS::"'a rel \<Rightarrow> 'a set \<Rightarrow> 'a set"
-where "AboveS r A \<equiv> {b \<in> Field r. \<forall>a \<in> A. b \<noteq> a \<and> (a,b) \<in> r}"
+definition AboveS :: "'a rel \<Rightarrow> 'a set \<Rightarrow> 'a set"
+  where "AboveS r A \<equiv> {b \<in> Field r. \<forall>a \<in> A. b \<noteq> a \<and> (a, b) \<in> r}"
 
 definition ofilter :: "'a rel \<Rightarrow> 'a set \<Rightarrow> bool"
-where "ofilter r A \<equiv> (A \<le> Field r) \<and> (\<forall>a \<in> A. under r a \<le> A)"
+  where "ofilter r A \<equiv> A \<subseteq> Field r \<and> (\<forall>a \<in> A. under r a \<subseteq> A)"
 
-text\<open>Note:  In the definitions of \<open>Above[S]\<close> and \<open>Under[S]\<close>,
-  we bounded comprehension by \<open>Field r\<close> in order to properly cover
-  the case of \<open>A\<close> being empty.\<close>
+text \<open>
+  Note: In the definitions of \<open>Above[S]\<close> and \<open>Under[S]\<close>, we bounded
+  comprehension by \<open>Field r\<close> in order to properly cover the case of \<open>A\<close> being
+  empty.
+\<close>
 
-lemma underS_subset_under: "underS r a \<le> under r a"
-by(auto simp add: underS_def under_def)
+lemma underS_subset_under: "underS r a \<subseteq> under r a"
+  by (auto simp add: underS_def under_def)
 
 lemma underS_notIn: "a \<notin> underS r a"
-by(simp add: underS_def)
+  by (simp add: underS_def)
 
-lemma Refl_under_in: "\<lbrakk>Refl r; a \<in> Field r\<rbrakk> \<Longrightarrow> a \<in> under r a"
-by(simp add: refl_on_def under_def)
+lemma Refl_under_in: "Refl r \<Longrightarrow> a \<in> Field r \<Longrightarrow> a \<in> under r a"
+  by (simp add: refl_on_def under_def)
 
-lemma AboveS_disjoint: "A Int (AboveS r A) = {}"
-by(auto simp add: AboveS_def)
+lemma AboveS_disjoint: "A \<inter> (AboveS r A) = {}"
+  by (auto simp add: AboveS_def)
 
 lemma in_AboveS_underS: "a \<in> Field r \<Longrightarrow> a \<in> AboveS r (underS r a)"
-by(auto simp add: AboveS_def underS_def)
+  by (auto simp add: AboveS_def underS_def)
 
-lemma Refl_under_underS:
-  assumes "Refl r" "a \<in> Field r"
-  shows "under r a = underS r a \<union> {a}"
-unfolding under_def underS_def
-using assms refl_on_def[of _ r] by fastforce
+lemma Refl_under_underS: "Refl r \<Longrightarrow> a \<in> Field r \<Longrightarrow> under r a = underS r a \<union> {a}"
+  unfolding under_def underS_def
+  using refl_on_def[of _ r] by fastforce
 
 lemma underS_empty: "a \<notin> Field r \<Longrightarrow> underS r a = {}"
-by (auto simp: Field_def underS_def)
+  by (auto simp: Field_def underS_def)
 
-lemma under_Field: "under r a \<le> Field r"
-by(unfold under_def Field_def, auto)
+lemma under_Field: "under r a \<subseteq> Field r"
+  by (auto simp: under_def Field_def)
 
-lemma underS_Field: "underS r a \<le> Field r"
-by(unfold underS_def Field_def, auto)
+lemma underS_Field: "underS r a \<subseteq> Field r"
+  by (auto simp: underS_def Field_def)
 
-lemma underS_Field2:
-"a \<in> Field r \<Longrightarrow> underS r a < Field r"
-using underS_notIn underS_Field by fast
+lemma underS_Field2: "a \<in> Field r \<Longrightarrow> underS r a \<subset> Field r"
+  using underS_notIn underS_Field by fast
 
-lemma underS_Field3:
-"Field r \<noteq> {} \<Longrightarrow> underS r a < Field r"
-by(cases "a \<in> Field r", simp add: underS_Field2, auto simp add: underS_empty)
+lemma underS_Field3: "Field r \<noteq> {} \<Longrightarrow> underS r a \<subset> Field r"
+  by (cases "a \<in> Field r") (auto simp: underS_Field2 underS_empty)
 
-lemma AboveS_Field: "AboveS r A \<le> Field r"
-by(unfold AboveS_def Field_def, auto)
+lemma AboveS_Field: "AboveS r A \<subseteq> Field r"
+  by (auto simp: AboveS_def Field_def)
 
 lemma under_incr:
-  assumes TRANS: "trans r" and REL: "(a,b) \<in> r"
-  shows "under r a \<le> under r b"
-proof(unfold under_def, auto)
-  fix x assume "(x,a) \<in> r"
-  with REL TRANS trans_def[of r]
-  show "(x,b) \<in> r" by blast
+  assumes "trans r"
+    and "(a, b) \<in> r"
+  shows "under r a \<subseteq> under r b"
+  unfolding under_def
+proof auto
+  fix x assume "(x, a) \<in> r"
+  with assms trans_def[of r] show "(x, b) \<in> r" by blast
 qed
 
 lemma underS_incr:
-assumes TRANS: "trans r" and ANTISYM: "antisym r" and
-        REL: "(a,b) \<in> r"
-shows "underS r a \<le> underS r b"
-proof(unfold underS_def, auto)
-  assume *: "b \<noteq> a" and **: "(b,a) \<in> r"
-  with ANTISYM antisym_def[of r] REL
-  show False by blast
+  assumes "trans r"
+    and "antisym r"
+    and ab: "(a, b) \<in> r"
+  shows "underS r a \<subseteq> underS r b"
+  unfolding underS_def
+proof auto
+  assume *: "b \<noteq> a" and **: "(b, a) \<in> r"
+  with \<open>antisym r\<close> antisym_def[of r] ab show False
+    by blast
 next
-  fix x assume "x \<noteq> a" "(x,a) \<in> r"
-  with REL TRANS trans_def[of r]
-  show "(x,b) \<in> r" by blast
+  fix x assume "x \<noteq> a" "(x, a) \<in> r"
+  with ab \<open>trans r\<close> trans_def[of r] show "(x, b) \<in> r"
+    by blast
 qed
 
 lemma underS_incl_iff:
-assumes LO: "Linear_order r" and
-        INa: "a \<in> Field r" and INb: "b \<in> Field r"
-shows "(underS r a \<le> underS r b) = ((a,b) \<in> r)"
+  assumes LO: "Linear_order r"
+    and INa: "a \<in> Field r"
+    and INb: "b \<in> Field r"
+  shows "underS r a \<subseteq> underS r b \<longleftrightarrow> (a, b) \<in> r"
+    (is "?lhs \<longleftrightarrow> ?rhs")
 proof
-  assume "(a,b) \<in> r"
-  thus "underS r a \<le> underS r b" using LO
-  by (simp add: order_on_defs underS_incr)
+  assume ?rhs
+  with \<open>Linear_order r\<close> show ?lhs
+    by (simp add: order_on_defs underS_incr)
 next
-  assume *: "underS r a \<le> underS r b"
-  {assume "a = b"
-   hence "(a,b) \<in> r" using assms
-   by (simp add: order_on_defs refl_on_def)
-  }
-  moreover
-  {assume "a \<noteq> b \<and> (b,a) \<in> r"
-   hence "b \<in> underS r a" unfolding underS_def by blast
-   hence "b \<in> underS r b" using * by blast
-   hence False by (simp add: underS_notIn)
-  }
-  ultimately
-  show "(a,b) \<in> r" using assms
-  order_on_defs[of "Field r" r] total_on_def[of "Field r" r] by blast
+  assume *: ?lhs
+  have "(a, b) \<in> r" if "a = b"
+    using assms that by (simp add: order_on_defs refl_on_def)
+  moreover have False if "a \<noteq> b" "(b, a) \<in> r"
+  proof -
+    from that have "b \<in> underS r a" unfolding underS_def by blast
+    with * have "b \<in> underS r b" by blast
+    then show ?thesis by (simp add: underS_notIn)
+  qed
+  ultimately show "(a,b) \<in> r"
+    using assms order_on_defs[of "Field r" r] total_on_def[of "Field r" r] by blast
 qed
 
 lemma finite_Linear_order_induct[consumes 3, case_names step]:
   assumes "Linear_order r"
-  and "x \<in> Field r"
-  and "finite r"
-  and step: "\<And>x. \<lbrakk>x \<in> Field r; \<And>y. y \<in> aboveS r x \<Longrightarrow> P y\<rbrakk> \<Longrightarrow> P x"
+    and "x \<in> Field r"
+    and "finite r"
+    and step: "\<And>x. x \<in> Field r \<Longrightarrow> (\<And>y. y \<in> aboveS r x \<Longrightarrow> P y) \<Longrightarrow> P x"
   shows "P x"
-using assms(2)
-proof(induct rule: wf_induct[of "r\<inverse> - Id"])
+  using assms(2)
+proof (induct rule: wf_induct[of "r\<inverse> - Id"])
+  case 1
   from assms(1,3) show "wf (r\<inverse> - Id)"
     using linear_order_on_well_order_on linear_order_on_converse
     unfolding well_order_on_def by blast
 next
-  case (2 x) then show ?case
-    by - (rule step; auto simp: aboveS_def intro: FieldI2)
+  case prems: (2 x)
+  show ?case
+    by (rule step) (use prems in \<open>auto simp: aboveS_def intro: FieldI2\<close>)
 qed
 
 
 subsection \<open>Variations on Well-Founded Relations\<close>
 
 text \<open>
-This subsection contains some variations of the results from @{theory Wellfounded}:
-\begin{itemize}
-\item means for slightly more direct definitions by well-founded recursion;
-\item variations of well-founded induction;
-\item means for proving a linear order to be a well-order.
-\end{itemize}
+  This subsection contains some variations of the results from @{theory Wellfounded}:
+    \<^item> means for slightly more direct definitions by well-founded recursion;
+    \<^item> variations of well-founded induction;
+    \<^item> means for proving a linear order to be a well-order.
 \<close>
 
 
 subsubsection \<open>Characterizations of well-foundedness\<close>
 
-text \<open>A transitive relation is well-founded iff it is ``locally'' well-founded,
-i.e., iff its restriction to the lower bounds of of any element is well-founded.\<close>
+text \<open>
+  A transitive relation is well-founded iff it is ``locally'' well-founded,
+  i.e., iff its restriction to the lower bounds of of any element is
+  well-founded.
+\<close>
 
 lemma trans_wf_iff:
-assumes "trans r"
-shows "wf r = (\<forall>a. wf(r Int (r^-1``{a} \<times> r^-1``{a})))"
-proof-
-  obtain R where R_def: "R = (\<lambda> a. r Int (r^-1``{a} \<times> r^-1``{a}))" by blast
-  {assume *: "wf r"
-   {fix a
-    have "wf(R a)"
-    using * R_def wf_subset[of r "R a"] by auto
-   }
-  }
-  (*  *)
+  assumes "trans r"
+  shows "wf r \<longleftrightarrow> (\<forall>a. wf (r \<inter> (r\<inverse>``{a} \<times> r\<inverse>``{a})))"
+proof -
+  define R where "R a = r \<inter> (r\<inverse>``{a} \<times> r\<inverse>``{a})" for a
+  have "wf (R a)" if "wf r" for a
+    using that R_def wf_subset[of r "R a"] by auto
   moreover
-  {assume *: "\<forall>a. wf(R a)"
-   have "wf r"
-   proof(unfold wf_def, clarify)
-     fix phi a
-     assume **: "\<forall>a. (\<forall>b. (b,a) \<in> r \<longrightarrow> phi b) \<longrightarrow> phi a"
-     obtain chi where chi_def: "chi = (\<lambda>b. (b,a) \<in> r \<longrightarrow> phi b)" by blast
-     with * have "wf (R a)" by auto
-     hence "(\<forall>b. (\<forall>c. (c,b) \<in> R a \<longrightarrow> chi c) \<longrightarrow> chi b) \<longrightarrow> (\<forall>b. chi b)"
-     unfolding wf_def by blast
-     moreover
-     have "\<forall>b. (\<forall>c. (c,b) \<in> R a \<longrightarrow> chi c) \<longrightarrow> chi b"
-     proof(auto simp add: chi_def R_def)
-       fix b
-       assume 1: "(b,a) \<in> r" and 2: "\<forall>c. (c, b) \<in> r \<and> (c, a) \<in> r \<longrightarrow> phi c"
-       hence "\<forall>c. (c, b) \<in> r \<longrightarrow> phi c"
-       using assms trans_def[of r] by blast
-       thus "phi b" using ** by blast
-     qed
-     ultimately have  "\<forall>b. chi b" by (rule mp)
-     with ** chi_def show "phi a" by blast
-   qed
-  }
-  ultimately show ?thesis using R_def by blast
+  have "wf r" if *: "\<forall>a. wf(R a)"
+    unfolding wf_def
+  proof clarify
+    fix phi a
+    assume **: "\<forall>a. (\<forall>b. (b, a) \<in> r \<longrightarrow> phi b) \<longrightarrow> phi a"
+    define chi where "chi b \<longleftrightarrow> (b, a) \<in> r \<longrightarrow> phi b" for b
+    with * have "wf (R a)" by auto
+    then have "(\<forall>b. (\<forall>c. (c, b) \<in> R a \<longrightarrow> chi c) \<longrightarrow> chi b) \<longrightarrow> (\<forall>b. chi b)"
+      unfolding wf_def by blast
+    also have "\<forall>b. (\<forall>c. (c, b) \<in> R a \<longrightarrow> chi c) \<longrightarrow> chi b"
+    proof (auto simp add: chi_def R_def)
+      fix b
+      assume "(b, a) \<in> r" and "\<forall>c. (c, b) \<in> r \<and> (c, a) \<in> r \<longrightarrow> phi c"
+      then have "\<forall>c. (c, b) \<in> r \<longrightarrow> phi c"
+        using assms trans_def[of r] by blast
+      with ** show "phi b" by blast
+    qed
+    finally have  "\<forall>b. chi b" .
+    with ** chi_def show "phi a" by blast
+  qed
+  ultimately show ?thesis unfolding R_def by blast
 qed
 
 text \<open>The next lemma is a variation of \<open>wf_eq_minimal\<close> from Wellfounded,
-allowing one to assume the set included in the field.\<close>
+  allowing one to assume the set included in the field.\<close>
 
-lemma wf_eq_minimal2:
-"wf r = (\<forall>A. A <= Field r \<and> A \<noteq> {} \<longrightarrow> (\<exists>a \<in> A. \<forall>a' \<in> A. \<not> (a',a) \<in> r))"
+lemma wf_eq_minimal2: "wf r \<longleftrightarrow> (\<forall>A. A \<subseteq> Field r \<and> A \<noteq> {} \<longrightarrow> (\<exists>a \<in> A. \<forall>a' \<in> A. (a', a) \<notin> r))"
 proof-
-  let ?phi = "\<lambda> A. A \<noteq> {} \<longrightarrow> (\<exists>a \<in> A. \<forall>a' \<in> A. \<not> (a',a) \<in> r)"
-  have "wf r = (\<forall>A. ?phi A)"
-  by (auto simp: ex_in_conv [THEN sym], erule wfE_min, assumption, blast)
-     (rule wfI_min, fast)
-  (*  *)
-  also have "(\<forall>A. ?phi A) = (\<forall>B \<le> Field r. ?phi B)"
+  let ?phi = "\<lambda>A. A \<noteq> {} \<longrightarrow> (\<exists>a \<in> A. \<forall>a' \<in> A. (a',a) \<notin> r)"
+  have "wf r \<longleftrightarrow> (\<forall>A. ?phi A)"
+    apply (auto simp: ex_in_conv [THEN sym])
+     apply (erule wfE_min)
+      apply assumption
+     apply blast
+    apply (rule wfI_min)
+    apply fast
+    done
+  also have "(\<forall>A. ?phi A) \<longleftrightarrow> (\<forall>B \<subseteq> Field r. ?phi B)"
   proof
     assume "\<forall>A. ?phi A"
-    thus "\<forall>B \<le> Field r. ?phi B" by simp
+    then show "\<forall>B \<subseteq> Field r. ?phi B" by simp
   next
-    assume *: "\<forall>B \<le> Field r. ?phi B"
+    assume *: "\<forall>B \<subseteq> Field r. ?phi B"
     show "\<forall>A. ?phi A"
-    proof(clarify)
-      fix A::"'a set" assume **: "A \<noteq> {}"
-      obtain B where B_def: "B = A Int (Field r)" by blast
-      show "\<exists>a \<in> A. \<forall>a' \<in> A. (a',a) \<notin> r"
-      proof(cases "B = {}")
-        assume Case1: "B = {}"
-        obtain a where 1: "a \<in> A \<and> a \<notin> Field r"
-        using ** Case1 unfolding B_def by blast
-        hence "\<forall>a' \<in> A. (a',a) \<notin> r" using 1 unfolding Field_def by blast
-        thus ?thesis using 1 by blast
+    proof clarify
+      fix A :: "'a set"
+      assume **: "A \<noteq> {}"
+      define B where "B = A \<inter> Field r"
+      show "\<exists>a \<in> A. \<forall>a' \<in> A. (a', a) \<notin> r"
+      proof (cases "B = {}")
+        case True
+        with ** obtain a where a: "a \<in> A" "a \<notin> Field r"
+          unfolding B_def by blast
+        with a have "\<forall>a' \<in> A. (a',a) \<notin> r"
+          unfolding Field_def by blast
+        with a show ?thesis by blast
       next
-        assume Case2: "B \<noteq> {}" have 1: "B \<le> Field r" unfolding B_def by blast
-        obtain a where 2: "a \<in> B \<and> (\<forall>a' \<in> B. (a',a) \<notin> r)"
-        using Case2 1 * by blast
-        have "\<forall>a' \<in> A. (a',a) \<notin> r"
-        proof(clarify)
-          fix a' assume "a' \<in> A" and **: "(a',a) \<in> r"
-          hence "a' \<in> B" unfolding B_def Field_def by blast
-          thus False using 2 ** by blast
+        case False
+        have "B \<subseteq> Field r" unfolding B_def by blast
+        with False * obtain a where a: "a \<in> B" "\<forall>a' \<in> B. (a', a) \<notin> r"
+          by blast
+        have "(a', a) \<notin> r" if "a' \<in> A" for a'
+        proof
+          assume a'a: "(a', a) \<in> r"
+          with that have "a' \<in> B" unfolding B_def Field_def by blast
+          with a a'a show False by blast
         qed
-        thus ?thesis using 2 unfolding B_def by blast
+        with a show ?thesis unfolding B_def by blast
       qed
     qed
   qed
@@ -441,58 +451,67 @@ qed
 
 subsubsection \<open>Characterizations of well-foundedness\<close>
 
-text \<open>The next lemma and its corollary enable one to prove that
-a linear order is a well-order in a way which is more standard than
-via well-foundedness of the strict version of the relation.\<close>
+text \<open>
+  The next lemma and its corollary enable one to prove that a linear order is
+  a well-order in a way which is more standard than via well-foundedness of
+  the strict version of the relation.
+\<close>
 
 lemma Linear_order_wf_diff_Id:
-assumes LI: "Linear_order r"
-shows "wf(r - Id) = (\<forall>A \<le> Field r. A \<noteq> {} \<longrightarrow> (\<exists>a \<in> A. \<forall>a' \<in> A. (a,a') \<in> r))"
-proof(cases "r \<le> Id")
-  assume Case1: "r \<le> Id"
-  hence temp: "r - Id = {}" by blast
-  hence "wf(r - Id)" by (simp add: temp)
-  moreover
-  {fix A assume *: "A \<le> Field r" and **: "A \<noteq> {}"
-   obtain a where 1: "r = {} \<or> r = {(a,a)}" using LI
-   unfolding order_on_defs using Case1 Total_subset_Id by auto
-   hence "A = {a} \<and> r = {(a,a)}" using * ** unfolding Field_def by blast
-   hence "\<exists>a \<in> A. \<forall>a' \<in> A. (a,a') \<in> r" using 1 by blast
-  }
+  assumes "Linear_order r"
+  shows "wf (r - Id) \<longleftrightarrow> (\<forall>A \<subseteq> Field r. A \<noteq> {} \<longrightarrow> (\<exists>a \<in> A. \<forall>a' \<in> A. (a, a') \<in> r))"
+proof (cases "r \<subseteq> Id")
+  case True
+  then have *: "r - Id = {}" by blast
+  have "wf (r - Id)" by (simp add: *)
+  moreover have "\<exists>a \<in> A. \<forall>a' \<in> A. (a, a') \<in> r"
+    if *: "A \<subseteq> Field r" and **: "A \<noteq> {}" for A
+  proof -
+    from \<open>Linear_order r\<close> True
+    obtain a where a: "r = {} \<or> r = {(a, a)}"
+      unfolding order_on_defs using Total_subset_Id [of r] by blast
+    with * ** have "A = {a} \<and> r = {(a, a)}"
+      unfolding Field_def by blast
+    with a show ?thesis by blast
+  qed
   ultimately show ?thesis by blast
 next
-  assume Case2: "\<not> r \<le> Id"
-  hence 1: "Field r = Field(r - Id)" using Total_Id_Field LI
-  unfolding order_on_defs by blast
+  case False
+  with \<open>Linear_order r\<close> have Field: "Field r = Field (r - Id)"
+    unfolding order_on_defs using Total_Id_Field [of r] by blast
   show ?thesis
   proof
-    assume *: "wf(r - Id)"
-    show "\<forall>A \<le> Field r. A \<noteq> {} \<longrightarrow> (\<exists>a \<in> A. \<forall>a' \<in> A. (a,a') \<in> r)"
-    proof(clarify)
-      fix A assume **: "A \<le> Field r" and ***: "A \<noteq> {}"
-      hence "\<exists>a \<in> A. \<forall>a' \<in> A. (a',a) \<notin> r - Id"
-      using 1 * unfolding wf_eq_minimal2 by simp
-      moreover have "\<forall>a \<in> A. \<forall>a' \<in> A. ((a,a') \<in> r) = ((a',a) \<notin> r - Id)"
-      using Linear_order_in_diff_Id[of r] ** LI by blast
-      ultimately show "\<exists>a \<in> A. \<forall>a' \<in> A. (a,a') \<in> r" by blast
+    assume *: "wf (r - Id)"
+    show "\<forall>A \<subseteq> Field r. A \<noteq> {} \<longrightarrow> (\<exists>a \<in> A. \<forall>a' \<in> A. (a, a') \<in> r)"
+    proof clarify
+      fix A
+      assume **: "A \<subseteq> Field r" and ***: "A \<noteq> {}"
+      then have "\<exists>a \<in> A. \<forall>a' \<in> A. (a',a) \<notin> r - Id"
+        using Field * unfolding wf_eq_minimal2 by simp
+      moreover have "\<forall>a \<in> A. \<forall>a' \<in> A. (a, a') \<in> r \<longleftrightarrow> (a', a) \<notin> r - Id"
+        using Linear_order_in_diff_Id [OF \<open>Linear_order r\<close>] ** by blast
+      ultimately show "\<exists>a \<in> A. \<forall>a' \<in> A. (a, a') \<in> r" by blast
     qed
   next
-    assume *: "\<forall>A \<le> Field r. A \<noteq> {} \<longrightarrow> (\<exists>a \<in> A. \<forall>a' \<in> A. (a,a') \<in> r)"
-    show "wf(r - Id)"
-    proof(unfold wf_eq_minimal2, clarify)
-      fix A assume **: "A \<le> Field(r - Id)" and ***: "A \<noteq> {}"
-      hence "\<exists>a \<in> A. \<forall>a' \<in> A. (a,a') \<in> r"
-      using 1 * by simp
-      moreover have "\<forall>a \<in> A. \<forall>a' \<in> A. ((a,a') \<in> r) = ((a',a) \<notin> r - Id)"
-      using Linear_order_in_diff_Id[of r] ** LI mono_Field[of "r - Id" r] by blast
-      ultimately show "\<exists>a \<in> A. \<forall>a' \<in> A. (a',a) \<notin> r - Id" by blast
+    assume *: "\<forall>A \<subseteq> Field r. A \<noteq> {} \<longrightarrow> (\<exists>a \<in> A. \<forall>a' \<in> A. (a, a') \<in> r)"
+    show "wf (r - Id)"
+      unfolding wf_eq_minimal2
+    proof clarify
+      fix A
+      assume **: "A \<subseteq> Field(r - Id)" and ***: "A \<noteq> {}"
+      then have "\<exists>a \<in> A. \<forall>a' \<in> A. (a,a') \<in> r"
+        using Field * by simp
+      moreover have "\<forall>a \<in> A. \<forall>a' \<in> A. (a, a') \<in> r \<longleftrightarrow> (a', a) \<notin> r - Id"
+        using Linear_order_in_diff_Id [OF \<open>Linear_order r\<close>] ** mono_Field[of "r - Id" r] by blast
+      ultimately show "\<exists>a \<in> A. \<forall>a' \<in> A. (a',a) \<notin> r - Id"
+        by blast
     qed
   qed
 qed
 
 corollary Linear_order_Well_order_iff:
-assumes "Linear_order r"
-shows "Well_order r = (\<forall>A \<le> Field r. A \<noteq> {} \<longrightarrow> (\<exists>a \<in> A. \<forall>a' \<in> A. (a,a') \<in> r))"
-using assms unfolding well_order_on_def using Linear_order_wf_diff_Id[of r] by blast
+  "Linear_order r \<Longrightarrow>
+    Well_order r \<longleftrightarrow> (\<forall>A \<subseteq> Field r. A \<noteq> {} \<longrightarrow> (\<exists>a \<in> A. \<forall>a' \<in> A. (a, a') \<in> r))"
+  unfolding well_order_on_def using Linear_order_wf_diff_Id[of r] by blast
 
 end
